proof/amd64/extracted/Keccak1600_Jazz.ec
@@ -449,7 +449,7 @@ module M = {
         w256 <@ __SHLQ_256 (w256, aT8);
         buf <- (buf + (8 - aT8));
         lEN <- (lEN - (8 - aT8));
-        aT8 <- 8;
+        aT <- (cUR + 8);
       } else {
         aT8 <- (aT - cUR);
         (buf, lEN, tRAIL, aT, w) <@ __m_ilen_read_upto8_at (buf, lEN, 
@@ -457,11 +457,7 @@ module M = {
         t128 <- (zeroextu128 w);
         w256 <- (VPBROADCAST_4u64 (truncateu64 t128));
         w256 <@ __SHLQ_256 (w256, aT8);
-        buf <- (buf + (8 - aT8));
-        lEN <- (lEN - (8 - aT8));
-        aT8 <- 8;
       }
-      aT <- (cUR + aT8);
     }
     return (buf, lEN, tRAIL, aT, w256);
   }
